Show WriterT is a retract of StateT

theories/Monads/Retract.v
@@ -1,9 +1,9 @@
 From Coq Require Import FunctionalExtensionality.
 
 From mtl.Classes Require Import All Retract.
-From mtl.Monads Require Import State Reader.
+From mtl.Monads Require Import State Reader Writer.
 
-Implicit Types s : Type.
+Implicit Types s e a : Type.
 Implicit Types m : Type -> Type.
 
 Module StateReader.
@@ -88,3 +88,85 @@ Qed.
 
 End StateReaderS.
 End StateReader.
+
+Module StateWriter.
+Section StateWriterS.
+
+Context {s : Type} `{Monoid s} {m : Type -> Type} `{Monad m}.
+
+Definition retract : forall a, StateT s m a -> WriterT s m a :=
+  fun a u => MkWriterT (runStateT u mempty >>= fun xz => pure (snd xz, fst xz)).
+
+Definition section : forall a, WriterT s m a -> StateT s m a :=
+  fun a u => MkStateT (fun z => runWriterT u >>= fun zx => pure (snd zx, (z ++ fst zx)%monoid)).
+
+Instance SemiIso_ {LM0 : LawfulMonoid s} {LM : LawfulMonad m} : SemiIso retract section.
+Proof.
+  red; intros; apply injective_runWriterT; intros; cbn.
+  rewrite bind_assoc; cbn.
+  transitivity (runWriterT u >>= pure).
+  - f_equal; apply functional_extensionality; intros [].
+    rewrite bind_pure_l, mappend_mempty_l; reflexivity.
+  - rewrite bind_pure_r; reflexivity.
+Qed.
+
+Instance MonadMorphism_section {LM0 : LawfulMonoid s} {LM : LawfulMonad m} :
+  @MonadMorphism _ _ (Monad_Retract retract section) _ section.
+Proof.
+  split; intros; apply injective_runStateT, functional_extensionality; intros; cbn.
+  - rewrite !bind_pure_l; cbn; rewrite mappend_mempty_r; reflexivity.
+  - rewrite !bind_assoc; f_equal; apply functional_extensionality; intros.
+    rewrite !bind_pure_l, !bind_assoc; f_equal; apply functional_extensionality; intros.
+    rewrite !bind_pure_l; cbn; rewrite mappend_mempty_l, mappend_assoc; reflexivity.
+Qed.
+
+(** The default instance of [Monad] for [ReaderT] coincides with the one
+    obtained by retraction. *)
+Theorem MonadRetract_eq {LM0 : LawfulMonoid s} {LM : LawfulMonad m} :
+  Monad_Retract retract section = Monad_WriterT.
+Proof.
+  unfold Monad_Retract, Monad_WriterT. f_equal.
+  all: repeat (apply functional_extensionality_dep; intros).
+  all: apply injective_runWriterT; intros; cbn.
+  - rewrite bind_pure_l; reflexivity.
+  - rewrite !bind_assoc; f_equal; apply functional_extensionality; intros [].
+    rewrite bind_pure_l, bind_assoc, mappend_mempty_l; cbn.
+    f_equal; apply functional_extensionality; intros [].
+    rewrite bind_pure_l; reflexivity.
+Qed.
+
+Instance MonadErrorMorphism_section {e} {LM0 : LawfulMonoid s}
+  {LM : LawfulMonad m} {ME : MonadError e m} {LME : LawfulMonadError e m} :
+  MonadErrorMorphismSection retract section.
+Proof.
+  split; intros; apply injective_runStateT, functional_extensionality; intros; cbn.
+  - rewrite !left_zero_throw; reflexivity.
+  - rewrite bind_assoc.
+    replace (fun xz => _ >>= _) with (fun az : a * s => pure (fst az, (x ++ snd az)%monoid)).
+    2: apply functional_extensionality; intros []; rewrite bind_pure_l; reflexivity.
+    pose proof natural_catch as NC. unfold mapM in NC. rewrite NC. clear NC.
+    f_equal. 2: apply functional_extensionality; intros.
+    all: rewrite bind_assoc; f_equal; apply functional_extensionality; intros;
+      rewrite bind_pure_l, mappend_mempty_l; reflexivity.
+Qed.
+
+(** The default instance of [MonadError] for [ReaderT] coincides with the one
+    obtained by retraction. *)
+Theorem MonadErrorRetract_eq {e} {LM0 : LawfulMonoid s}
+  {LM : LawfulMonad m} `{MonadError e m} {LME : LawfulMonadError e m} :
+  MonadError_Retract retract section = MonadError_WriterT.
+Proof.
+  unfold MonadError_Retract, MonadError_WriterT. f_equal.
+  all: repeat (apply functional_extensionality_dep; intros).
+  all: apply injective_runWriterT; intros; cbn.
+  - rewrite left_zero_throw; reflexivity.
+  - pose proof natural_catch as NC. unfold mapM in NC. rewrite NC. clear NC.
+    f_equal. 2: apply functional_extensionality; intros.
+    all: rewrite bind_assoc.
+    all: replace (fun zx => _) with (fun zx : s * x => pure zx : m (s * x)%type)
+      by (apply functional_extensionality; intros []; rewrite bind_pure_l, mappend_mempty_l; reflexivity).
+    all: rewrite bind_pure_r; reflexivity.
+Qed.
+
+End StateWriterS.
+End StateWriter.
